Foundations.thy
@@ -1,0 +1,15 @@
+(*<*)
+theory Foundations
+  imports 
+    Pure
+begin
+(*>*)
+
+
+text \<open>introducing essential concepts like LTS, equivalence, HML, (relational equivalence definitions?)
+- mention sources (Ben / Max Pohlmann?)\<close>
+
+
+(*<*)
+end
+(*>*)
